minor fix

src/certigrad/aevb/transformations.lean
@@ -13,33 +13,37 @@ namespace aevb
 
 open graph list tactic certigrad.tactic
 
+meta def prove_transformation (e : pexpr) :=
+do whnf_target,
+  [tgt, idx, H_at_idx, θ] ← intro_lst [`tgt, `idx, `H_at_idx, `θ] | failed,
+  forall_idxs prove_model_base
+              (do H_at_idx ← get_local `H_at_idx,
+                  mk_app `and.right [H_at_idx] >>= note `H_tgt_eq,
+                  H_tgt_eq_type ← get_local `H_tgt_eq >>= infer_type,
+                  s ← join_user_simp_lemmas true [`cgsimp],
+                  (H_tgt_eq_new_type, pr) ← simplify s H_tgt_eq_type {},
+                  get_local `H_tgt_eq >>= λ H_tgt_eq, replace_hyp H_tgt_eq H_tgt_eq_new_type pr,
+                  get_local `H_tgt_eq >>= subst,
+                  to_expr e >>= apply,
+                  all_goals (cgsimp >> try prove_is_mvn_integrable >> try T.prove_preconditions))
+              idx
+
 lemma integrate_kl_sound (a : arch) (ws : weights a) (x_data : T [a^.n_in, a^.n_x]) :
 let g₀ : graph := graph_naive a x_data, fdict : env := mk_input_dict ws g₀ in
 ∀ (tgt : reference) (idx : ℕ) (H_at_idx : at_idx g₀^.targets idx tgt) (θ : T tgt.2),
 E (graph.to_dist (λ m, ⟦sum_costs m (integrate_kl g₀)^.costs⟧) (env.insert tgt θ fdict) (integrate_kl g₀)^.nodes) dvec.head
 =
-E (graph.to_dist (λ m, ⟦sum_costs m g₀^.costs⟧) (env.insert tgt θ fdict) g₀^.nodes) dvec.head := sorry
-/-
-by do whnf_target,
-      [tgt, idx, H_at_idx, θ] ← intros | failed,
-      forall_idxs prove_model_base (do
-         to_expr ```(integrate_mvn_iso_kl_correct (ID.str label.encoding_loss) [ID.str label.decoding_loss] (graph_naive a x_data)^.nodes) >>= apply,
-         all_goals (cgsimp >> try prove_is_mvn_integrable >> try T.prove_preconditions)) idx
--/
+E (graph.to_dist (λ m, ⟦sum_costs m g₀^.costs⟧) (env.insert tgt θ fdict) g₀^.nodes) dvec.head :=
+by prove_transformation ```(integrate_mvn_iso_kl_correct (ID.str label.encoding_loss) [ID.str label.decoding_loss] (graph_naive a x_data)^.nodes)
 
 lemma reparam_sound (a : arch) (ws : weights a) (x_data : T [a^.n_in, a^.n_x]) :
 let g₁ : graph := integrate_kl (graph_naive a x_data), fdict : env := mk_input_dict ws g₁ in
 ∀ (tgt : reference) (idx : ℕ) (H_at_idx : at_idx g₁^.targets idx tgt) (θ : T tgt.2),
 E (graph.to_dist (λ m, ⟦sum_costs m (reparam g₁)^.costs⟧) (env.insert tgt θ fdict) (reparam g₁)^.nodes) dvec.head
 =
-E (graph.to_dist (λ m, ⟦sum_costs m g₁^.costs⟧) (env.insert tgt θ fdict) g₁^.nodes) dvec.head := sorry
-/-
-by do whnf_target,
-      [tgt, idx, H_at_idx, θ] ← intros | failed,
-      forall_idxs prove_model_base (do
-         to_expr ```(reparameterize_correct _ (integrate_kl $ graph_naive a x_data)^.nodes _ (ID.str label.ε, [a^.nz, a^.bs])) >>= apply,
-         all_goals cgsimp) idx
--/
+E (graph.to_dist (λ m, ⟦sum_costs m g₁^.costs⟧) (env.insert tgt θ fdict) g₁^.nodes) dvec.head :=
+by prove_transformation ```(reparameterize_correct [ID.str label.encoding_loss, ID.str label.decoding_loss]
+                                                  (integrate_kl $ graph_naive a x_data)^.nodes _ (ID.str label.ε, [a^.nz, a^.bs]))
 
 -- TODO(dhs): this is annoying, rw and simp should whnf the let
 lemma aevb_transformations_sound {a : arch} (ws : weights a) (x_data : T [a^.n_in, a^.n_x]) :
@@ -53,7 +57,6 @@ whnf_target,
 intros tgt idx H_at_idx θ,
 note H₁ := @reparam_sound a ws x_data tgt idx,
 note H₂ := @integrate_kl_sound a ws x_data tgt idx,
-dsimp at *,
 simp only [naive_aevb_as_graph] at *,
 erw [H₁, H₂],
 all_goals { assumption }
